Bf/Part2.lean
@@ -2,28 +2,55 @@ import Bf.Part1
 
 
 
-/-! # Abstract runtime: non-trivial code and monads -/
-namespace Zen.Train.Bf
+/-! # Runtime
+
+## Loop limit
+
+We're going to have a potentially infinite loop detection mechanism. So let's discuss that first.
+
+As we execute `Ast` code, we will find `Ast.block`-s causing us to run their bodies (potientially)
+multiple times. As we do this, for each block we (re-)execute we will maintain two important pieces
+of information.
+
+- `oldVal`: the cell value used for the non-zero check the last time we entered this block;
+- `count`: the number of times the cell value we checked was **not** smaller than the old value.
+
+For instance:
+
+| current cell |           comment            | `oldVal` | `count` |
+| -----------: | :--------------------------: | -------: | ------: |
+|         `15` |        entering block        |     `15` |     `0` |
+|         `10` | `10 < 15`, `count` unchanged |     `10` |     `0` |
+|         `11` | `11 ≥ 10`, `count` increased |     `11` |     `1` |
+|         `11` | `11 ≥ 11`, `count` increased |     `11` |     `2` |
+|          `7` |          you get it          |      `7` |     `2` |
+|          `2` |             ...              |      `2` |     `2` |
+|          `0` |             done             |     none |    none |
+
+The actual runtime will have an optional loop limit that will throw an error if `count` becomes
+greater than that limit (if any).
+-/
+namespace Zen.Train.Bf.Rt
 
 
 
-inductive Ast.Frame
-| seq : (array : Array Ast) → Fin array.size → Frame
-| block (oldVal : Nat) (count : Nat) : Ast → Frame
-
-abbrev Ast.Frames := List Ast.Frame
-
-
-
-inductive Rt.Error
+/-- Errors that running brainfuck code can throw. -/
+inductive Error
+/-- General-purpose string error. -/
 | text : String → Error
+/-- Loop limit reached, see module-level documentation for details. -/
 | loopLimit : (limit : Nat) → (count : Nat) → limit < count → Error
+/-- A failed `Ast.check`.
+
+Stores the check's message, its expected value, the actual value, and a proof that they are
+different.
+-/
 | checkFailed : String → (exp : Nat) → (val : Nat) → exp ≠ val → Error
 
-namespace Rt.Error
+namespace Error
 
-def toString : Rt.Error → String
-| text msg => s!"error: {msg}"
+def toString : Error → String
+| text msg => s!"{msg}"
 | loopLimit limit count _ => s!"\
   potential infinite loop detected \
   after {count} non-decreasing iterations \
@@ -34,142 +61,376 @@ def toString : Rt.Error → String
 
 instance instToString : ToString Error :=
   ⟨toString⟩
-end Rt.Error
+
+end Error
 
 
 
-class Rt.Spec (Mon : Type → Type u) where
-  op : Ast.Op → Mon Unit
-  seff : Ast.Seff → Mon Unit
-  check : Ast.Check → Mon Unit
-  isZeroCurr : Mon Bool
-  getCurr : Mon Nat
-  getLoopLimit : Mon $ Option Nat
-  fail : Rt.Error → Mon α
+/-! Time to do something!
+
+Define `Mem` which is just our basic brainfuck memory. It stores two things:
+
+- the actualy memory as an `Array Nat`;
+- a pointer to the current cell.
+
+I'm not giving you the type for the pointer. Just know that you will probably want to use the
+following functions at some point.
+-/
+#check Array.get
+#check Array.set
+
+/-! And no, you're not allowed to use those. -/
+#check Array.get!
+#check Array.set!
+
+/-! Also, please make the default constructor private with `private <ident> ::` between the `where`
+and the fields:
+
+```lean
+structure Mem where
+private mkRaw ::
+  <fields>
+```
+-/
+
+
+section sol!
+structure Mem where
+private mkRaw ::
+  mem : Array Nat
+  ptr : Fin mem.size
+end sol!
+
+namespace Mem
+
+/-!
+**NB**: remember that autocompletion is your friend, and so is Lean's documentation:
+
+- <https://leanprover-community.github.io/mathlib4_docs>
+
+
+Write the following functions, their semantics should be straightforward from their signatures.
+-/
+
+/-!
+**NB**: when you need to prove something simple, try `by simp` in case it works.
+-/
+section sol!
+def mk (capacity : Nat := 123) : Mem where
+  mem := Array.mkEmpty capacity |>.push 0
+  ptr := ⟨0, by simp⟩
+end sol!
+/-- info: Zen.Train.Bf.Rt.Mem.mk (capacity : Nat := 123) : Mem -/
+#guard_msgs in #check mk
 
 
 
-section
-variable
-  ⦃Mon : Type → Type u⦄
-  [Monad Mon]
-  [R : Rt.Spec Mon]
+variable (self : Mem)
 
-partial def Ast.runWith (stack : Ast.Frames) : Ast → Mon Unit
-| .op o => do
-  R.op o
-  goUp stack
-| .seff s => do
-  R.seff s
-  goUp stack
-| .check c => do
-  R.check c
-  goUp stack
-| .block b => do
-  if ← R.isZeroCurr then goUp stack else
-    let val ← R.getCurr
-    b.runWith (.block val 0 b :: stack)
-| .seq s =>
-  if h : 0 < s.size then
-    let stack := .seq s ⟨0, h⟩ :: stack
-    s[0].runWith stack
-  else goUp stack
-where
-  goUp : Ast.Frames → Mon Unit
-  | [] => return ()
-  | .seq s idx :: stack =>
-    let idx := idx.val + 1
-    if h : idx < s.size then
-      let stack := .seq s ⟨idx, h⟩ :: stack
-      s[idx].runWith stack
-    else
-      goUp stack
-  | .block oldVal count body :: stack => do
-    if ← R.isZeroCurr then goUp stack else
-      let val ← R.getCurr
-      let count := if val < oldVal then count else count.succ
-      let loopLimit ← R.getLoopLimit
-      if let some limit := loopLimit then
-        if h_lt : limit < count then
-          Rt.Error.loopLimit limit count h_lt
-          |> R.fail
-      body.runWith (.block val count body :: stack)
+def mapCurr (f : Nat → Nat) : Mem :=
+  let val := f self.mem[self.ptr]
+  let mem := self.mem.set self.ptr val
+  let tmp : mem.size = self.mem.size :=
+    by simp [mem]
+  ⟨mem, tmp ▸ self.ptr⟩
 
-partial def Ast.runWithDbg [MonadLiftT IO Mon] (stack : Ast.Frames) : Ast → Mon Unit
-| .op o => do
-  println! "op {o}"
-  R.op o
-  goUp stack
-| .seff s => do
-  println! "seff {s}"
-  R.seff s
-  goUp stack
-| .check c => do
-  println! "check {c}"
-  R.check c
-  goUp stack
-| .block b => do
-  println! "entering block"
-  if ← R.isZeroCurr then goUp stack else
-    let val ← R.getCurr
-    b.runWithDbg (.block val 0 b :: stack)
-| .seq s => do
-  println! "entering sequence"
-  if h : 0 < s.size then
-    let stack := .seq s ⟨0, h⟩ :: stack
-    println! "-> {s[0]}"
-    s[0].runWithDbg stack
+
+
+section sol!
+def getCurr : Nat :=
+  self.mem[self.ptr]
+end sol!
+/-- info: Zen.Train.Bf.Rt.Mem.getCurr (self : Mem) : Nat -/
+#guard_msgs in #check getCurr
+
+
+
+/-! Note: `Ast.mvl` does nothing if we're pointing to the first cell of the array. (Maybe look at
+what `Nat` subtraction does.)
+
+Also, for no reason at all, maybe take a look at these.
+-/
+#checkout Nat.lt_of_le_of_lt
+#checkout Nat.pred_le
+section sol!
+def mvl : Mem := {self with
+  ptr := ⟨
+    self.ptr - 1,
+    Nat.lt_of_le_of_lt self.ptr.val.pred_le self.ptr.isLt,
+  ⟩
+}
+end sol!
+/-- info: Zen.Train.Bf.Rt.Mem.mvl (self : Mem) : Mem -/
+#guard_msgs in #check mvl
+
+
+
+/-! This next one is more advanced, take a look but we go over it together.
+
+We will use the following two theorems though, you can check them out.
+-/
+#checkout Array.size_push
+#checkout Nat.succ_lt_succ
+section sol!
+def mvr : Mem :=
+  if isLt : self.ptr.val + 1 < self.mem.size
+  then { self with ptr := ⟨self.ptr.val + 1, isLt⟩ }
   else
-    println! "empty sequence, going up"
-    goUp stack
+    let mem := self.mem.push 0
+    { self with
+        mem
+        ptr := ⟨self.ptr.val + 1, by simp [mem, Array.size_push, Nat.succ_lt_succ]⟩
+    }
+end sol!
+/-- info: Zen.Train.Bf.Rt.Mem.mvr (self : Mem) : Mem -/
+#guard_msgs in #check mvr
+
+
+
+def applyOp : Ast.Op → Mem
+| .mvr => self.mvr
+| .mvl => self.mvl
+| .inc => self.mapCurr Nat.succ
+| .dec => self.mapCurr Nat.pred
+
+end Mem
+
+
+
+structure Config where
+  /-- If false, ignore debug messages. -/
+  dbg : Bool
+  /-- If false, ignore checks. -/
+  check : Bool
+  /-- Optional loop limit, see module-level documentation. -/
+  loopLimit : Option Nat
+
+namespace Config
+protected def default : Config where
+  dbg := true
+  check := true
+  loopLimit := some 123
+
+instance instInhabited : Inhabited Config where
+  default := Config.default
+end Config
+
+
+
+/-- The full state, extends `Mem` with some configuration and the inputs/outputs. -/
+structure State extends Mem, Config where
+private mkRaw ::
+  inputs : List Nat
+  outputs : Array Nat
+
+namespace State
+
+def mk (inputs : List Nat) (capa : Nat := 123) (config : Config := default) : State where
+  toMem := Mem.mk capa
+  toConfig := config
+  inputs := inputs
+  outputs := #[]
+
+variable (self : State)
+
+/-! Notice how we can use `Config`'s fields as `State` fields. -/
+
+def withConfig (config : Config) : State :=
+  {self with toConfig := config}
+def withDbg (dbg : Bool) : State :=
+  {self with dbg}
+def withCheck (check : Bool) : State :=
+  {self with check}
+def withLoopLimit (loopLimit : Nat) : State :=
+  {self with loopLimit}
+def withNoLoopLimit : State :=
+  {self with loopLimit := none}
+
+/-! Here are a few functions to write so that you don't fall asleed. -/
+section sol!
+private def liftMemFun (f : Mem → Mem) : State → State
+| self => {self with toMem := f self.toMem}
+
+def emit (n : Nat) : State :=
+  {self with outputs := self.outputs.push n}
+
+def drainInput : Nat × State :=
+  match self.inputs with
+  | [] => (0, self)
+  | nxt::inputs => (nxt, {self with inputs})
+
+def drainOutputs : Array Nat × State :=
+  (self.outputs, {self with outputs := #[]})
+end sol!
+
+/-- info: Zen.Train.Bf.Rt.State.liftMemFun (f : Mem → Mem) : State → State -/
+#guard_msgs in #check liftMemFun
+/-- info: Zen.Train.Bf.Rt.State.emit (self : State) (n : Nat) : State -/
+#guard_msgs in #check emit
+/-- info: Zen.Train.Bf.Rt.State.drainInput (self : State) : Nat × State -/
+#guard_msgs in #check drainInput
+/-- info: Zen.Train.Bf.Rt.State.drainOutputs (self : State) : Array Nat × State -/
+#guard_msgs in #check drainOutputs
+
+
+
+def mapCurr f := liftMemFun fun m => m.mapCurr f
+def applyOp o := liftMemFun fun m => m.applyOp o
+def mvl := liftMemFun .mvl
+def mvr := liftMemFun .mvr
+def getCurr := self.toMem.getCurr
+
+end State
+
+
+
+/-- Output extraction strategy.
+
+Users will provide a value of this type to run on the outputs of their execution once it's over.
+-/
+inductive Extract : Type → Type 1
+/-- Extracts nothing. -/
+| unit : Extract Unit
+/-- Extracts the array of outputs without doing anything. -/
+| array : Extract (Array Nat)
+/-- Yields the first output, if any. -/
+| head? : Extract (Option Nat)
+/-- Yields the first output, fails if none. -/
+| head! : Extract Nat
+/-- Folds over the outputs, allowed to fail. -/
+| tryFold : α → (α → Nat → Except Error α) → Extract α
+
+namespace Extract
+
+abbrev Out : Extract α → Type := 𝕂 α
+
+/-! Let's write more functions 🐙 -/
+
+section sol!
+def fold (init : α) (f : α → Nat → α) : Extract α :=
+  tryFold init (f · · |> .ok)
+end sol!
+/-- info: Zen.Train.Bf.Rt.Extract.fold {α : Type} (init : α) (f : α → Nat → α) : Extract α -/
+#guard_msgs in #check fold
+
+section sol!
+/- I know, you haven't seen monads yet, we'll see this version after the interlude. -/
+def apply : (self : Extract α) → Array Nat → Except Error α
+| unit, _ => return ()
+| array, a => return a
+| head?, a =>
+  if h : 0 < a.size
+  then return a[0]
+  else return none
+| head!, a => do
+  if h : 0 < a.size
+  then return a[0]
+  else .error <| .text "[bf] failed to extract output `head!`, no output available"
+| tryFold init f, l => do
+  let mut res := init
+  for n in l do
+    res ← f res n
+  return res
+  -- -- alternatively just
+  -- l.foldlM f init
+
+def apply' : Extract α → Array Nat → Except Error α
+| unit, _ => .ok ()
+| array, a => .ok a
+| head?, a =>
+  if h : 0 < a.size then .ok a[0] else .ok none
+| head!, a => do
+  if h : 0 < a.size then .ok a[0] else
+    .error <| .text "[bf] failed to extract output `head!`, no output available"
+| tryFold init f, l =>
+  applyTryFold init f l.data
 where
-  goUp : Ast.Frames → Mon Unit
-  | [] => return ()
-  | .seq s idx :: stack => do
-    let idx := idx.val + 1
-    if h : idx < s.size then
-      let stack := .seq s ⟨idx, h⟩ :: stack
-      println! "going down ({stack.length})"
-      s[idx].runWithDbg stack
+  applyTryFold {α : Type} init f : List Nat → Except Error α
+  | [] => .ok init
+  | hd::tl =>
+    match f init hd with
+    | .ok init => applyTryFold init f tl
+    | .error e => .error e
+end sol!
+/-- info:
+Zen.Train.Bf.Rt.Extract.apply {α : Type} (self : Extract α) : Array Nat → Except Error α
+-/
+#guard_msgs in #check apply
+
+
+/-! Write `apply!`, which is defined as `Option.get! ∘ Except.toOption ∘ self.apply`. -/
+section sol!
+def apply! [Inhabited α] (self : Extract α) :=
+  Option.get! ∘ Except.toOption ∘ self.apply
+end sol!
+
+
+
+/-- Extracts the sum of all the outputs. -/
+def sum (init : Nat := 0) : Extract Nat :=
+  fold init Nat.add
+
+/-- info:
+- sum #[0, 1, 2, 3] => 6
+- sum #[] => 0
+-/
+#guard_msgs in #eval do
+  let data := #[0, 1, 2, 3]
+  println! "- sum {data} => {sum.apply! data}"
+  println! "- sum #[] => {sum.apply! #[]}"
+
+
+
+/-- String list extraction, where non-char values are interpreted as separators. -/
+def string : Extract (Array String) :=
+  fold #[] combine
+where
+  combine stringArray n :=
+    let c := Char.ofNat n
+    if c.val = 0 then
+      -- v~~~~ **we need this**
+      if h : stringArray.size ≠ 0 then
+        if let "" := stringArray.last
+        then stringArray
+        else stringArray.push ""
+      else
+        stringArray
     else
-      println! "going up ({stack.length})"
-      goUp stack
-  | .block oldVal count body :: stack => do
-    println! "going up block"
-    if ← R.isZeroCurr then goUp stack else
-      let val ← R.getCurr
-      let count := if val < oldVal then count else count.succ
-      let loopLimit ← R.getLoopLimit
-      if let some limit := loopLimit then
-        if h_lt : limit < count then
-          Rt.Error.loopLimit limit count h_lt
-          |> R.fail
-      body.runWithDbg (.block val count body :: stack)
+      let (curr, stringArray) :=
+        -- v~~~~ **we need this too**
+        if h : stringArray.size ≠ 0
+        then stringArray.pop'
+        else ("", stringArray)
+      curr.push c |> stringArray.push
 
+/-- info:
+first result:
+  `I 🖤 猫`
+second result:
+  `I 🖤 猫`
+  `next bit`
+third result:
+  `I 🖤 猫`
+  `next bit`
+  `and then`
+  `finally`
+-/
+#guard_msgs in #eval do
+  let chars := "I 🖤 猫".data.map Char.toNat
+  println! "first result:"
+  for bit in string.apply! chars.toArray do
+    println! "  `{bit}`"
+  let chars :=
+    chars ++ [0] ++ ("next bit".data.map Char.toNat)
+  println! "second result:"
+  for bit in string.apply! chars.toArray do
+    println! "  `{bit}`"
+  let chars :=
+    chars
+    ++ [20^10] ++ ("and then".data.map Char.toNat)
+    ++ [20130531] ++ [52016027] ++ ("finally".data.map Char.toNat)
+  println! "third result:"
+  for bit in string.apply! chars.toArray do
+    println! "  `{bit}`"
 
-abbrev Rt.Spec.runCode : Ast → Mon Unit :=
-  Ast.runWith []
-end
-
-
-structure Rt : Type 1 where
-  Mon : Type → Type
-  instMonad : Monad Mon
-  instSpec : Rt.Spec Mon
-
-namespace Rt
-variable (self : Rt)
-
-/-! Make internal instances visible. -/
-
-instance instMonadMon : Monad self.Mon := self.instMonad
-instance instSpecMon : Spec self.Mon := self.instSpec
-
-/-- Runs an ast on some runtime. -/
-def run (a : Ast) : self.Mon Unit :=
-  a.runWith []
-
-end Rt
-
-def Ast.runIn : (R : Rt) → Ast → R.Mon Unit :=
-  Rt.run
+end Extract
