Bf/Part3.lean
@@ -2,301 +2,416 @@ import Bf.Part2
 
 
 
-/-! # Concretizing the runtime -/
+/-! # Abstract runtime: non-trivial code and monads -/
 namespace Zen.Train.Bf
 
 
-structure Rt.Basic.Mem where
-private mkRaw ::
-  mem : Array Nat
-  ptr : Fin mem.size
 
-namespace Rt.Basic.Mem
+/-! Whatever the effect of the `Op`-s, `Seff`-s and `Check`-s, the nodes of the AST (`Ast.block` and
+`Ast.seq`) have the same semantics as long as we can check the value of the current cell.
 
-def mk (capa : Nat := 123) : Mem where
-  mem := Array.mkEmpty capa |>.push 0
-  ptr := ⟨0, by simp⟩
+Let's write an abstract interpreter that handles the nodes and defers to semantics to define later
+-/
 
-variable (self : Mem)
 
-def mapCurr (f : Nat → Nat) : Mem :=
-  let val := f self.mem[self.ptr]
-  let mem := self.mem.set self.ptr val
-  let tmp : mem.size = self.mem.size :=
-    by simp [mem]
-  ⟨mem, tmp ▸ self.ptr⟩
+namespace Rt
 
-def getCurr : Nat :=
-  self.mem[self.ptr]
 
-def mvl : Mem := {self with
-  ptr := ⟨self.ptr - 1, Nat.lt_of_le_of_lt self.ptr.val.pred_le self.ptr.isLt⟩
-}
+/-- Frames of the abstract interpreter.
 
-def mvr : Mem :=
-  if isLt : self.ptr.val + 1 < self.mem.size
-  then { self with ptr := ⟨self.ptr.val + 1, isLt⟩ }
-  else
-    let mem := self.mem.push 0
-    {self with mem, ptr := ⟨self.ptr.val + 1, by
-      simp [mem, Array.size_push, Nat.succ_lt_succ]
-    ⟩}
-
-def applyOp : Ast.Op → Mem
-| .mvr => self.mvr
-| .mvl => self.mvl
-| .inc => self.mapCurr Nat.succ
-| .dec => self.mapCurr Nat.pred
-
-end Rt.Basic.Mem
+The interpreter is going to be tailrec, obviously, so we have to handle the `Stack` (list of
+`Frame`s) by hand. The frames store the information needed to deal with the nodes of the AST
+(`Ast.seq` and `Ast.block`). When we interpret an `Ast.seq` for instance, we need to *go down*
+(execute) the first element, and once that's over we *go up* (look in the stack) to find the frame
+with the information needed to run the second element (if any), and so on.
+-/
+inductive Frame
+/--
+Stores the elements of the sequence, and a pointer telling us which elements we are currently in. So
+when we go up the stack and see `Frame.seq elems i` we know we just executed the `elems[i]`; we now
+need to check whether we're done with the sequence, and if not update the frame to point to the next
+element and go down that element.
+-/
+| seq : (array : Array Ast) → Fin array.size → Frame
+/--
+Stores the `oldVal` and `count` quantities discussed in the documentation of module `Bf.Part2`, and
+the body of the block.
+-/
+| block (oldVal : Nat) (count : Nat) : Ast → Frame
 
 
 
-structure Rt.Basic.State extends Rt.Basic.Mem where
-private mkRaw ::
-  dbg : Bool
-  check : Bool
-  loopLimit : Option Nat
-  inputs : List Nat
-  outputs : Array Nat
-
-namespace Rt.Basic.State
-
-def mk (inputs : List Nat) (capa : Nat := 123) : State where
-  toMem := Mem.mk capa
-  dbg := true
-  check := true
-  loopLimit := some 123
-  inputs := inputs
-  outputs := #[]
-
-private def liftMemFun (f : Mem → Mem) : State → State
-| self => {self with toMem := f self.toMem}
-
-variable (self : State)
-
-def emit (n : Nat) : State :=
-  {self with outputs := self.outputs.push n}
-
-def drainInput : Nat × State :=
-  match self.inputs with
-  | [] => (0, self)
-  | nxt::inputs => (nxt, {self with inputs})
-
-def mapCurr f := liftMemFun fun m => m.mapCurr f
-def applyOp o := liftMemFun fun m => m.applyOp o
-def mvl := liftMemFun .mvl
-def mvr := liftMemFun .mvr
-def getCurr := self.toMem.getCurr
-
-end Rt.Basic.State
+/-- A list of `Frame`s. -/
+abbrev Stack := List Frame
 
 
 
-inductive Rt.Extract : Type → Type 1
-| unit : Extract Unit
-| array : Extract (Array Nat)
-| head? : Extract (Option Nat)
-| head! : Extract Nat
-| tryFold : α → (α → Nat → Except Rt.Error α) → Extract α
+/-- Abstracts over the runtime memory and the semantics of the operations. -/
+class Spec (Mon : Type → Type u) where
+  /-- Applies an operator. -/
+  op : Ast.Op → Mon Unit
+  /-- Applies a side-effect. -/
+  seff : Ast.Seff → Mon Unit
+  /-- Runs a check. -/
+  check : Ast.Check → Mon Unit
+  /-- Yields the current cell value. -/
+  getCurr : Mon Nat
+  /-- The loop limit, see `Frame`'s documentation for details. Note that it does not need to be
+  static. -/
+  getLoopLimit : Mon $ Option Nat
+  /-- Throws an error. -/
+  throw : Error → Mon α
 
-namespace Rt.Extract
+namespace Spec
 
-protected abbrev Out (_ : Extract α) : Type := α
+variable {Mon : Type → Type u} [Monad Mon]
 
-instance instCoeSort : CoeSort (Extract α) Type :=
-  ⟨𝕂 α⟩
+def isZeroCurr [Self : Spec Mon] : Mon Bool :=
+  --      vvv~~~~~ `Functor.map`, comes for free as `Monad Mon` implies `Functor Mon`
+  (· = 0) <$> Self.getCurr
 
-def fold (init : α) (f : α → Nat → α) : Extract α :=
-  tryFold init (f · · |> .ok)
-
-
-def apply : (self : Extract α) → Array Nat → Except Rt.Error α
-| unit, _ => return ()
-| array, a => return a
-| head?, a =>
-  if h : 0 < a.size
-  then return a[0]
-  else return none
-| head!, a => do
-  if h : 0 < a.size
-  then return a[0]
-  else .error <| .text "[bf] failed to extract output `head!`, no output available"
-| tryFold init f, l => do
-  let mut res := init
-  for n in l do
-    res ← f res n
-  return res
-  -- -- alternatively just
-  -- l.foldlM f init
-
-def apply! (self : Extract α) [Inhabited α] :=
-  (self.apply · |>.toOption |>.get!)
+#checkout Functor
 
 
 
-/-- String extraction, where non-char values are interpreted as separators. -/
-def string : Extract (Array String) :=
-  fold #[] combine
+namespace run.Test
+/-! Time to do something!
+
+Write a `scoped instance TestRt : Spec (StateT State IO)`.
+
+We will use it for testing in a few moments, I **strongly** suggest you take a look at my version
+once you're done to avoid having problems in both `TestRt` and what we're about to test with it.
+
+Alternatively, consider calling your version `TestRt'` and using my version once you're done writing
+yours.
+-/
+
+#checkout StateT
+
+scoped instance TestRt : Spec (StateT State IO) where
+  op op := do
+    let state ← get
+    set (state.applyOp op)
+  seff
+  | .out => fun s => return ((), s.emit s.getCurr)
+  | .inp => fun s =>
+    let (val, s) := s.drainInput
+    return ((), s.mapCurr (𝕂 val))
+  | .dbg msg => println! msg
+  check
+  | .chk exp msg, s => do
+    let val := s.getCurr
+    if val ≠ exp
+    then IO.throwServerError s!"check failed: {val} ≠ {exp}, {msg}"
+    else return ((), s)
+  getCurr := do
+    return (← get).getCurr
+  getLoopLimit := return some 1
+  throw e := do
+    IO.throwServerError s!"{e}"
+end run.Test
+
+
+/-! Write `def runWithStack [Self : Spec Mon] : Stack → Ast → Mon Unit`.
+
+(I omitted `Mon` and its `Monad` instance in this signature as they are variables.)
+
+(Strong) suggestion: use `where` to define a helper `goUp : Stack → Mon Unit`.
+
+```
+def runWithStack ...
+  ...
 where
-  combine stringArray n :=
-    let c := Char.ofNat n
-    if c.val = 0 then
-      if h : stringArray.size ≠ 0 then
-        if let "" := stringArray.last
-        then stringArray
-        else stringArray.push ""
-      else
-        stringArray
+  goUp : Stack → Mon Unit
+    ...
+```
+-/
+
+section sol!
+partial def runWithStack [Self : Spec Mon] (stack : Stack) : Ast → Mon Unit
+| .op o => do
+  Self.op o
+  goUp stack
+| .seff s => do
+  Self.seff s
+  goUp stack
+| .check c => do
+  Self.check c
+  goUp stack
+| .block b => do
+  if ← Self.isZeroCurr then goUp stack else
+    let val ← Self.getCurr
+    Self.runWithStack (.block val 0 b :: stack) b
+| .seq s =>
+  if h : 0 < s.size then
+    let stack := .seq s ⟨0, h⟩ :: stack
+    Self.runWithStack stack s[0]
+  else goUp stack
+where
+  goUp : Stack → Mon Unit
+  | [] => return ()
+  | .seq s idx :: stack =>
+    let idx := idx.val + 1
+    if h : idx < s.size then
+      let stack := .seq s ⟨idx, h⟩ :: stack
+      Self.runWithStack stack s[idx]
     else
-      let (curr, stringArray) :=
-        if h : stringArray.size ≠ 0
-        then stringArray.pop'
-        else ("", stringArray)
-      curr.push c |> stringArray.push
+      goUp stack
+  | .block oldVal count body :: stack => do
+    if ← Self.isZeroCurr then goUp stack else
+      let val ← Self.getCurr
+      let count := if val < oldVal then count else count.succ
+      let loopLimit ← Self.getLoopLimit
+      if let some limit := loopLimit then
+        if h_lt : limit < count then
+          Error.loopLimit limit count h_lt
+          |> Self.throw
+      Self.runWithStack (.block val count body :: stack) body
+end sol!
 
 /-- info:
-first result:
-  `I 🖤 猫`
-second result:
-  `I 🖤 猫`
-  `next bit`
-third result:
-  `I 🖤 猫`
-  `next bit`
-  `and then`
-  `finally`
+Zen.Train.Bf.Rt.Spec.runWithStack.{u} {Mon : Type → Type u} [Monad Mon] [Self : Spec Mon] (stack : Stack) :
+  Ast → Mon Unit
+-/
+#guard_msgs in #check runWithStack
+
+
+
+abbrev justRun [Self : Spec Mon] : Ast → Mon Unit :=
+  Self.runWithStack []
+
+
+
+namespace run.Test
+def run (ast : Ast) (inputs : List Nat := []) : IO (Array Nat) := do
+  let state := State.mk inputs
+  let (_, state) ← TestRt.justRun ast state
+  return state.outputs
+
+/-- error:
+potential infinite loop detected after 2 non-decreasing iterations (limit is 1)
+-/
+#guard_msgs(error, drop info) in #eval do
+  -- `+[]` (infinite loop)
+  let ast := Ast.seq #[.inc, .blockSeq #[]]
+  run ast
+
+/--
+info: done, let's fail now
+---
+error: check failed: 0 ≠ 3, expected failure 🐙
 -/
 #guard_msgs in #eval do
-  let chars := "I 🖤 猫".data.map Char.toNat
-  println! "first result:"
-  for bit in string.apply! chars.toArray do
-    println! "  `{bit}`"
-  let chars :=
-    chars ++ [0] ++ ("next bit".data.map Char.toNat)
-  println! "second result:"
-  for bit in string.apply! chars.toArray do
-    println! "  `{bit}`"
-  let chars :=
-    chars
-    ++ [2013420531] ++ ("and then".data.map Char.toNat)
-    ++ [20130531] ++ [52016027] ++ ("finally".data.map Char.toNat)
-  println! "third result:"
-  for bit in string.apply! chars.toArray do
-    println! "  `{bit}`"
-
-def sum (init : Nat := 0) : Extract Nat :=
-  fold init Nat.add
+  -- `>+++<` (move right, add 3, move left)
+  let ast := Ast.seq #[
+    .chk 0 "should be 0",
+    .mvr,
+    .chk 0 "should be 0 too",
+    .inc, .inc, .inc,
+    .chk 3 "should be 3",
+    .mvl,
+    .chk 0 "should still be 0",
+    .dbg "done, let's fail now",
+    .chk 3 "expected failure 🐙"
+  ]
+  run ast
 
 /-- info:
-- sum #[0, 1, 2, 3] => 6
-- sum #[] => 0
+copying left
+not done
+not done
+not done
+done
+#[0, 3]
 -/
 #guard_msgs in #eval do
-  let data := #[0, 1, 2, 3]
-  println! "- sum {data} => {sum.apply! data}"
-  println! "- sum #[] => {sum.apply! #[]}"
+  -- `,[->+<].>.` (read input and copy it to the next cell)
+  let ast := Ast.seq #[
+    .inp,
+    .dbg "copying left",
+    .blockSeq #[.dbg "not done", .dec, .mvr, .inc, .mvl],
+    .dbg "done",
+    .out, .mvr, .out
+  ]
+  --       v~~ loop limit is `1`, but the loop checks decreasing values
+  run ast [3]
 
-end Rt.Extract
+end run.Test
 
-
-
-structure Rt.Extract' : Type 1 where
-private mkRaw ::
-  Out : Type
-  isInhabitedOut : Inhabited Out
-  isToExprOut : Lean.ToExpr Out
-  extract : Extract Out
-
-namespace Rt.Extract'
-def mk [Inhabited α] [Lean.ToExpr α] (extract : Extract α) : Extract' where
-  Out := α
-  isInhabitedOut := inferInstance
-  isToExprOut := inferInstance
-  extract := extract
-
-instance instInhabited : Inhabited Extract' where
-  default := mk Extract.array
-
-variable (self : Extract')
-
-instance instInhabitedOut : Inhabited self.Out := self.isInhabitedOut
-instance instToExprOut : Lean.ToExpr self.Out := self.isToExprOut
-
-def apply := self.extract.apply
-def apply! := self.extract.apply!
-end Rt.Extract'
+end Spec
 
 
 
-def Rt.Extract.hideType
-  [Inhabited α] [Lean.ToExpr α]
-  (self : Extract α)
-: Extract' :=
-  Extract'.mk self
+/-! Great so at this point we have
+
+- a notion of `State` (with internal `Mem`ory), and
+- a `Spec`ification with an abstract `Spec.run` function
+
+we need to have a clean way to deal with errors and monad-related stuff.
+
+We're going to define a `BfT` error/state monad transformer 🙀. Remember
+
+- state monad transformer: `abbrev StateM σ M α := σ → M (α × σ)`, no way to report errors without
+  making some assumption on `M`;
+- error monad: `inductive Except ε α | ok α | error ε`.
+
+(Try to) define `BfT M α`, the error/state monad with fixed state `State`.
+
+Note that, as is often the case we want to be able to access the state even when an error is
+produced. It's useful for debugging.
+-/
+
+section sol!
+/-!
+It **might** be a good idea to introduce a first definition, potentially called `BfT.Res`.
+-/
+
+inductive BfT.Res (α : Type)
+| ok : α → State → Res α
+| error : Error → State → Res α
+
+abbrev BfT (M : Type → Type) (α : Type) :=
+  State → M (BfT.Res α)
+end sol!
 
 
 
+/-! Great, make sure you have my version now. -/
 
-inductive Rt.BfT.Res (α : Type)
-| ok : α → Basic.State → Res α
-| error : Error → Basic.State → Res α
+namespace BfT.Res
+/-! Is `BfT.Res` a (reasonable) monad?
 
-namespace Rt.BfT.Res
+Is there a `bind`-like operation that would make sense here?
+-/
+
+section sol!
 instance instFunctor : Functor Res where
   map
-    | f, ok val s => ok (f val) s
-    | _, error e s => error e s
+  | f, ok val s => ok (f val) s
+  | _, error e s => error e s
 
 def map (f : α → β) (self : Res α) :=
   f <$> self
-end Rt.BfT.Res
+end sol!
+end BfT.Res
 
-abbrev Rt.BfT (M : Type → Type) (α : Type) :=
-  Basic.State → M (BfT.Res α)
 
-namespace Rt.BfT
+
+namespace BfT
 variable {M : Type → Type} [Monad M]
 
-def fail : Error → BfT M α :=
+
+/-! Let's write a bunch of functions 🐙 -/
+
+section sol!
+def throw : Error → BfT M α :=
   (.error · · |> pure)
+end sol!
+/-- info:
+Zen.Train.Bf.Rt.BfT.throw {M : Type → Type} [Monad M] {α : Type} : Error → BfT M α
+-/
+#guard_msgs in #check throw
 
-def loopLimitFail : (limit : Nat) → (count : Nat) → limit < count → BfT M α :=
-  (.loopLimit · · · |> fail)
+section sol!
+def throwLoopLimit : (limit : Nat) → (count : Nat) → limit < count → BfT M α :=
+  (.loopLimit · · · |> throw)
+end sol!
+/-- info:
+Zen.Train.Bf.Rt.BfT.throwLoopLimit {M : Type → Type} [Monad M] {α : Type} (limit count : Nat) : limit < count → BfT M α
+-/
+#guard_msgs in #check throwLoopLimit
 
-def checkFail (msg : String) (exp val : Nat) (h_ne : exp ≠ val) : BfT M α :=
-  fail <| .checkFailed msg exp val h_ne
+section sol!
+def throwCheckFailed (msg : String) (exp val : Nat) (h_ne : exp ≠ val) : BfT M α :=
+  throw <| .checkFailed msg exp val h_ne
+end sol!
+/-- info:
+Zen.Train.Bf.Rt.BfT.throwCheckFailed {M : Type → Type} [Monad M] {α : Type} (msg : String) (exp val : Nat)
+  (h_ne : exp ≠ val) : BfT M α
+-/
+#guard_msgs in #check throwCheckFailed
 
-def getState : BfT M Basic.State
+section sol!
+def getState : BfT M State
 | state => return .ok state state
+end sol!
+/-- info:
+Zen.Train.Bf.Rt.BfT.getState {M : Type → Type} [Monad M] : BfT M State
+-/
+#guard_msgs in #check getState
 
-def setState : Basic.State → BfT M Unit
+section sol!
+def setState : State → BfT M Unit
 | state, _ => return .ok () state
+end sol!
+/-- info:
+Zen.Train.Bf.Rt.BfT.setState {M : Type → Type} [Monad M] : State → BfT M Unit
+-/
+#guard_msgs in #check setState
 
-def mapMStateAnd : (Basic.State → M (α × Basic.State)) → BfT M α
+section sol!
+def mapMStateAnd : (State → M (α × State)) → BfT M α
 | f, state => do
   let (res, state) ← f state
   return .ok res state
+end sol!
+/-- info:
+Zen.Train.Bf.Rt.BfT.mapMStateAnd {M : Type → Type} [Monad M] {α : Type} : (State → M (α × State)) → BfT M α
+-/
+#guard_msgs in #check mapMStateAnd
 
-def mapMState (f : Basic.State → M Basic.State) : BfT M Unit :=
+section sol!
+def mapMState (f : State → M State) : BfT M Unit :=
   mapMStateAnd fun state => do
     return ((), ← f state)
+end sol!
+/-- info:
+Zen.Train.Bf.Rt.BfT.mapMState {M : Type → Type} [Monad M] (f : State → M State) : BfT M Unit
+-/
+#guard_msgs in #check mapMState
 
-def stateDoM (f : Basic.State → M α) : BfT M α :=
+section sol!
+def stateDoM (f : State → M α) : BfT M α :=
   mapMStateAnd fun state => do
     return (← f state, state)
+end sol!
+/-- info:
+Zen.Train.Bf.Rt.BfT.stateDoM {M : Type → Type} [Monad M] {α : Type} (f : State → M α) : BfT M α
+-/
+#guard_msgs in #check stateDoM
 
-def mapStateAnd (f : Basic.State → α × Basic.State) : BfT M α :=
+section sol!
+def mapStateAnd (f : State → α × State) : BfT M α :=
   mapMStateAnd (return f ·)
+end sol!
+/-- info:
+Zen.Train.Bf.Rt.BfT.mapStateAnd {M : Type → Type} [Monad M] {α : Type} (f : State → α × State) : BfT M α
+-/
+#guard_msgs in #check mapStateAnd
 
-def mapState (f : Basic.State → Basic.State) : BfT M Unit :=
+section sol!
+def mapState (f : State → State) : BfT M Unit :=
   mapMState (return f ·)
+end sol!
+/-- info:
+Zen.Train.Bf.Rt.BfT.mapState {M : Type → Type} [Monad M] (f : State → State) : BfT M Unit
+-/
+#guard_msgs in #check mapState
 
-def stateDo (f : Basic.State → α) : BfT M α :=
+section sol!
+def stateDo (f : State → α) : BfT M α :=
   stateDoM (return f ·)
+end sol!
+/-- info:
+Zen.Train.Bf.Rt.BfT.stateDo {M : Type → Type} [Monad M] {α : Type} (f : State → α) : BfT M α
+-/
+#guard_msgs in #check stateDo
 
 
 
+/-! Time for `Monad (BfT M)`! -/
+
+section sol!
 protected def pure (a : α) : BfT M α
 | state => return .ok a state
 
@@ -309,15 +424,23 @@ protected def bind (code : BfT M α) (f : α → BfT M β) : BfT M β
 instance instMonad : Monad (BfT M) where
   pure := BfT.pure
   bind := BfT.bind
+end sol!
 
+
+
+/-! And the appropriate `MonadLift` instance. -/
+
+section sol!
 instance instMonadLift : MonadLift M (BfT M) where
   monadLift m state := do
     let val ← m
     return .ok val state
+end sol!
 
 
 
-open Basic (State)
+/-! Lifting/defining useful state manipulation functions. -/
+section liftStateFunctions
 
 def getCurr : BfT M Nat :=
   stateDo State.getCurr
@@ -332,16 +455,16 @@ def getLoopLimit : BfT M (Option Nat) :=
   stateDo fun s => s.loopLimit
 
 def withDbg (dbg : Bool) : BfT M Unit :=
-  mapState ({· with dbg})
+  mapState fun s => s.withDbg dbg
 
 def withCheck (check : Bool) : BfT M Unit :=
-  mapState ({· with check})
+  mapState fun s => s.withCheck check
 
 def withLoopLimit (loopLimit : Nat) : BfT M Unit :=
-  mapState ({· with loopLimit})
+  mapState fun s => s.withLoopLimit loopLimit
 
 def withNoLoopLimit : BfT M Unit :=
-  mapState ({· with loopLimit := none})
+  mapState State.withNoLoopLimit
 
 def handleOp (op : Ast.Op) : BfT M Unit :=
   mapState fun s => s.applyOp op
@@ -353,7 +476,27 @@ def drainInput : BfT M Nat :=
   mapStateAnd fun s => s.drainInput
 
 def drainOutputs : BfT M (Array Nat) :=
-  mapStateAnd fun s => (s.outputs, {s with outputs := Array.mkEmpty 123})
+  mapStateAnd fun s => s.drainOutputs
+
+end liftStateFunctions
+
+
+
+/-! Define the following:
+
+- `handleCheck : Ast.Check → BfT M Unit`, self-explanatory;
+- `handleSeff : Ast.Seff → BfT M Unit`: ignores `Seff.dbg`-s;
+- `handleSeff ... : Ast.Seff → BfT M Unit`: handles `Seff.dbg`-s with `println!`.
+-/
+
+section sol!
+def handleCheck : Ast.Check → BfT M Unit
+| .chk exp msg => do
+  let self ← getState
+  if self.check then
+    let val ← getCurr
+    if h_ne : exp ≠ val then
+      throwCheckFailed msg exp val h_ne
 
 def handleSeff : Ast.Seff → BfT M Unit
 | .out => do
@@ -370,112 +513,82 @@ def handleSeffIO [MonadLiftT IO M] : Ast.Seff → BfT M Unit
   if (←getState).dbg then
     liftM (println! msg)
 | seff => handleSeff seff
+end sol!
 
-def handleCheck : Ast.Check → BfT M Unit
-| .chk exp msg => do
-  let self ← getState
-  if self.check then
-    let val ← getCurr
-    if h_ne : exp ≠ val then
-      checkFail msg exp val h_ne
+end BfT
 
 
-instance instSpec : Spec (BfT M) where
-  op := handleOp
-  seff := handleSeff
-  check := handleCheck
-  isZeroCurr := isZeroCurr
-  getCurr := getCurr
-  getLoopLimit := getLoopLimit
-  fail := fail
 
-instance instSpecIO [MonadLiftT IO M] : Spec (BfT M) :=
-  {instSpec with seff := handleSeffIO}
+/-! `Spec` instances! -/
 
-/-- info: done #[2] -/
+protected instance NoIO [Monad M] : Spec (BfT M) where
+  op := BfT.handleOp
+  seff := BfT.handleSeff
+  check := BfT.handleCheck
+  getCurr := BfT.getCurr
+  getLoopLimit := BfT.getLoopLimit
+  throw := BfT.throw
+
+protected instance IO [Monad M] [MonadLiftT IO M] : Spec (BfT M) :=
+  {Rt.NoIO with seff := BfT.handleSeffIO}
+
+/-- info:
+done
+memory: #[0, 2]
+#[2]
+-/
 #guard_msgs in #eval do
   let ast := Ast.Test.val1
-  let blah := instSpecIO.runCode ast $ Rt.Basic.State.mk []
-  match ← blah with
-  | .ok _ s => return s.outputs
+  let res := Rt.IO.justRun ast $ State.mk []
+  match ← res with
+  | .ok _ s =>
+    println! "memory: {s.mem}"
+    return s.outputs
   | .error e s =>
     println! "something went wrong, memory state is {s.mem}@{s.ptr}"
     IO.throwServerError e.toString
 
 
 
+namespace Spec
+variable [Monad M]
 
-def run
+def justExe
   (S : Spec (BfT M)) (code : Ast) (ex : Extract α)
 : BfT M α := do
-  S.runCode code
-  match ex.apply (← drainOutputs) with
+  S.justRun code
+  match ex.apply (← BfT.drainOutputs) with
   | .ok res => return res
-  | .error e => S.fail e
+  | .error e => S.throw e
 
-def justRun
-  [Inhabited α]
-  (S : Spec (BfT M)) (code : Ast) (inputs : List Nat) (ex : Extract α)
+def exe
+  (S : Spec (BfT M)) (code : Ast) (inputs : List Nat) (ex : Extract α) (config := Config.default)
 : M (BfT.Res α) := do
-  Basic.State.mk inputs |> run S code ex
+  State.mk inputs (config := config) |> S.justExe code ex
 
-def justRun!
+def exe!
   [Inhabited α]
-  (S : Spec (BfT M)) (code : Ast) (inputs : List Nat) (ex : Extract α)
+  (S : Spec (BfT M)) (code : Ast) (inputs : List Nat) (ex : Extract α) (config := Config.default)
 : M α := do
-  match ← justRun S code inputs ex with
+  match ← S.exe code inputs ex config with
   | .ok res _ => return res
   | .error err _ => panic! err.toString
-
-def justRunToExpr
-  [Inhabited α] [Lean.ToExpr α]
-  (S : Spec (BfT M)) (code : Ast) (inputs : List Nat) (ex : Extract α)
-: M (BfT.Res Lean.Expr) := do
-  let res ← justRun S code inputs ex
-  return Lean.ToExpr.toExpr <$> res
-
-end Rt.BfT
-
-namespace Rt.NoIO
-variable {M : Type → Type} [Monad M] [MonadLiftT IO M] [Inhabited α] [Lean.ToExpr α]
-  (code : Ast) (inputs : List Nat) (ex : Extract α)
-
-def run : BfT M α :=
-  Rt.BfT.run Rt.BfT.instSpec code ex
-def justRun : M (Rt.BfT.Res α) :=
-  Rt.BfT.justRun Rt.BfT.instSpec code inputs ex
-def justRun! : M α :=
-  Rt.BfT.justRun! Rt.BfT.instSpec code inputs ex
-def justRunToExpr : M (Rt.BfT.Res Lean.Expr) :=
-  Rt.BfT.justRunToExpr Rt.BfT.instSpec code inputs ex
-end Rt.NoIO
-
-namespace Rt.IO
-variable {M : Type → Type} [Monad M] [MonadLiftT IO M] [Inhabited α] [Lean.ToExpr α]
-  (code : Ast) (inputs : List Nat) (ex : Extract α)
-
-def run : BfT M α :=
-  Rt.BfT.run Rt.BfT.instSpecIO code ex
-def justRun : M (Rt.BfT.Res α) :=
-  Rt.BfT.justRun Rt.BfT.instSpecIO code inputs ex
-def justRun! : M α :=
-  Rt.BfT.justRun! Rt.BfT.instSpecIO code inputs ex
-def justRunToExpr : M (Rt.BfT.Res Lean.Expr) :=
-  Rt.BfT.justRunToExpr Rt.BfT.instSpecIO code inputs ex
-end Rt.IO
+end Spec
 
 
 
 /-- info: done #[2, 8] -/
 #guard_msgs in #eval
-  Rt.IO.justRun! (M := IO) (Ast.Test.val1 ++ .mvr ++ .inp ++ .inc ++ .out) [7] .array
+  Rt.IO.exe! (M := IO) (Ast.Test.val1 ++ .mvr ++ .inp ++ .inc ++ .out) [7] .array
 
 
-abbrev Rt.BfM :=
+abbrev BfM :=
   BfT Id
 
-abbrev Rt.BfIO :=
+abbrev BfIO :=
   BfT IO
+
+end Rt
 
 
 
@@ -485,24 +598,24 @@ variable
   (self : Ast) (inputs : List Nat) (ex : Rt.Extract α)
 
 def evalTo : Rt.BfT.Res α :=
-  Rt.NoIO.justRun (M := Id) self inputs ex
+  Rt.NoIO.exe (M := Id) self inputs ex
 def eval : Rt.BfT.Res (Array Nat) :=
-  Rt.NoIO.justRun (M := Id) self inputs .array
+  Rt.NoIO.exe (M := Id) self inputs .array
 
 def evalTo! : α :=
-  Rt.NoIO.justRun! (M := Id) self inputs ex
+  Rt.NoIO.exe! (M := Id) self inputs ex
 def eval! : Array Nat :=
-  Rt.NoIO.justRun! (M := Id) self inputs .array
+  Rt.NoIO.exe! (M := Id) self inputs .array
 
 def evalIOTo : IO (Rt.BfT.Res α) :=
-  Rt.IO.justRun (M := IO) self inputs ex
+  Rt.IO.exe (M := IO) self inputs ex
 def evalIO : IO (Rt.BfT.Res (Array Nat)) :=
-  Rt.IO.justRun (M := IO) self inputs .array
+  Rt.IO.exe (M := IO) self inputs .array
 
 def evalIOTo! : IO α :=
-  Rt.IO.justRun! (M := IO) self inputs ex
+  Rt.IO.exe! (M := IO) self inputs ex
 def evalIO! : IO (Array Nat) :=
-  Rt.IO.justRun! (M := IO) self inputs .array
+  Rt.IO.exe! (M := IO) self inputs .array
 end Ast
 
 
