Bf.lean
@@ -2,6 +2,7 @@ import Bf.Init
 import Bf.Part0
 import Bf.Part1
 import Bf.Part2
+import Bf.Part2Interlude
 import Bf.Part3
 import Bf.Part4
 
