Bf/Part2Interlude.lean
@@ -1,0 +1,454 @@
+import Bf.Init
+
+
+
+/-! # Monads and `do` notation -/
+namespace Zen.Train.Trash.MonadsAndDo
+
+
+
+/-! A monad wraps values of any type `α` and is equipped with two operations. -/
+
+/-- For instance: -/
+abbrev Just : Type → Type := id
+
+#check Just
+
+namespace Just
+def get : Just α → α := id
+
+/-- Injects a value into the monad. -/
+protected def pure (val : α) : Just α :=
+  val
+
+/-- Given a `Just α`-value, apply a function to the inner `α` that returns a `Just β`-value. -/
+protected def bind (justVal : Just α) (f : α → Just β) : Just β :=
+  f justVal
+
+
+/-! Now check this out.
+
+```
+let mut val := 7
+if 0 < val then
+  val := val - 1
+val := val % 2
+```
+
+This is obviously not compatible with a pure language. Or is it?
+-/
+
+def encodeLetMut (val : Nat) : Just Nat :=
+  Just.pure val
+  |>.bind (fun val =>
+    let val := if 0 < val then val - 1 else val
+    Just.pure val
+  )
+  |>.bind (fun val =>
+    Just.pure (val % 2)
+  )
+
+example : encodeLetMut 7 = Just.pure 0 := rfl
+example : encodeLetMut 0 = Just.pure 0 := rfl
+example : encodeLetMut 8 = Just.pure 1 := rfl
+
+
+
+/-! This is basically how the `do` notation works for `Monad`s. -/
+
+#checkout Monad
+
+instance instMonad : Monad Just where
+  pure := Just.pure
+  bind := Just.bind
+
+def doLetMut (val : Nat) : Just Nat := do
+  let mut val := val
+  if 0 < val then val := val - 1
+  return val % 2 -- same as `pure (val % 2)`
+
+end Just
+
+
+
+/-! ## `do` notation: `←`
+
+Define an option type `Opt : Type → Type` with variants `non`e and `som`e.
+
+(To avoid clashing with Lean's `Option` type).
+-/
+
+section sol!
+inductive Opt (α : Type) : Type
+| non
+| som : α → Opt α
+end sol!
+
+#check Opt.non
+#check Opt.som
+
+namespace Opt
+
+/-! Write a `ToString` instance for `Opt`. -/
+section sol!
+instance instToString [ToString α] : ToString (Opt α) where
+  toString
+    | non => "none"
+    | som a => toString a
+end sol!
+
+/-! Write a `Monad` instance for `Opt`. -/
+section sol!
+instance instMonad : Monad Opt where
+  pure := som
+  bind
+  | non, _ => non
+  | som a, f => f a
+end sol!
+
+
+
+/-! We can use `←` to "access the value", *i.e.* trigger a bind. -/
+
+def map (a? : Opt α) (f : α → β) : Opt β := do
+  let a ← a? -- using `←` instead of `:=`
+  return f a -- again, `return <term>` is just `pure (<term>)`
+
+def map' (a? : Opt α) (f : α → β) : Opt β := do
+  -- you can also do this
+  return f (← a?)
+
+def mapWithBind (a? : Opt α) (f : α → β) : Opt β :=
+  -- `bind a? (pure ∘ f)`, but let's write it with the infix `>>=` bind operator to look cool
+  a? >>= pure ∘ f
+
+
+def demo (a? : Opt Nat) : Opt Nat := do
+  if let 0 ← a?
+  then non else
+    match ← a? with
+    | 0 => panic! "unreachable!"
+    | 7 => return 7
+    | _ => non
+
+/-! `#eval` actually takes a term of type `IO α`, and `IO` is a monad. -/
+#checkout IO
+#checkout IO.println
+
+#eval do
+  let mut val := demo (som 0)
+  -- same as `IO.println` but takes an interpolated string
+  println! "{val}"
+  -- has type `IO Unit`, `do` notation lets us chain `M Unit` expressions when `M` is a monad
+
+  val := demo (som 1) -- also has type `M Unit` (`IO Unit`, here)
+  println! "{val}"
+  val := demo (som 7)
+  println! "{val}"
+  return ()
+
+end Opt
+
+
+
+/-! ## State monads
+
+Exercise / discussion
+
+In a purely functional language, how would you write a function that produces some result `α` but
+also
+
+- just reads some state?
+- reads and write some state?
+-/
+
+structure State where
+  counter : Nat
+
+section sol!
+def justReads (params : Nat) (state : State) : Nat :=
+  params + state.counter
+
+-- alternatively
+def justReads' (params : Nat) : State → Nat :=
+  fun state => params + state.counter
+
+def readsWrites (params : Nat) (state : State) : Nat × State :=
+  let out := justReads params state
+  let state := { state with counter := state.counter + 1 }
+  (out, state)
+
+-- alternatively
+def readsWrites' (params : Nat) : State → Nat × State :=
+  fun state =>
+    let out := justReads params state
+    let state := { state with counter := state.counter + 1 }
+    (out, state)
+end sol!
+
+
+
+/-! What would be the corresponding monads `ReadM` and `WriteM` for some generic state type `σ`? -/
+
+section sol!
+abbrev ReadM (σ : Type) (α : Type) : Type :=
+  σ → α
+
+abbrev WriteM (σ : Type) (α : Type) : Type :=
+  σ → α × σ
+  -- same as `ReadM σ (α × σ)`
+end sol!
+
+
+
+/-! Now just write `Monad` instances for them. -/
+
+section sol!
+instance ReadM.instMonad : Monad (ReadM σ) where
+  pure a _state := a
+  bind a? f? state :=
+    let a := a? state
+    f? a state
+
+instance WriteM.instMonad : Monad (WriteM σ) where
+  pure := Prod.mk
+  bind a? f? state :=
+    let (a, state) := a? state
+    f? a state
+end sol!
+
+
+
+/-! Awesome, now we can define a few helpers. -/
+
+def ReadM.get : ReadM σ σ
+| state => state
+
+def WriteM.get : WriteM σ σ
+| state => (state, state)
+
+def WriteM.set : σ → WriteM σ Unit
+| newState, _oldState => ((), newState)
+
+
+
+abbrev Log := Array String
+
+def WriteM.demo (n : Nat) : WriteM Log Nat := do
+  log "checking if `n` is zero"
+  if n = 0 then
+    log' "`n` is zero!"
+    return n
+  else
+    log "`n` is not zero, modulo-2-ing it"
+    return n % 2
+where
+  log (msg : String) : WriteM Log Unit := do
+    let log ← get
+    set <| log.push msg
+  /-- Arguably simpler, arguably not as fancy. -/
+  log' (msg : String) : WriteM Log Unit
+    | log => ((), log.push msg)
+
+
+/-! Write `WriteM.runDemo : IO Unit` that runs `WriteM.demo` on some inputs, shows the results and
+log for each call.
+-/
+
+section sol!
+def WriteM.runDemo : IO Unit := do
+  let state := #[]
+  let (res, state) := demo 7 state
+  println! "demo 7"
+  -- so, turns out we can also `for`-iterate on collections when in a monad 😺
+  -- see the `ForIn` class for details
+  for line in state do
+    println! "- {line}"
+  println! "↦ {res}"
+  println! ""
+
+  let state := #[]
+  let (res, state) := demo 0 state
+  println! "demo 7"
+  for line in state do
+    println! "- {line}"
+  println! "↦ {res}"
+  println! ""
+
+  let state := #[]
+  let (res, state) := demo 10 state
+  println! "demo 7"
+  for line in state do
+    println! "- {line}"
+  println! "↦ {res}"
+end sol!
+
+#eval WriteM.runDemo
+
+end MonadsAndDo
+
+
+
+/-! The `Just` monad is called `Id` in Lean. -/
+#checkout Id
+#checkout (inferInstance : Monad Id) -- would fail if no `Monad Id` instances existed
+
+
+
+/-! The cool thing is that we can run imperative-looking code whenever we want with `Id`. -/
+#checkout Id.run
+
+/-- Array pretty-printer (`pp`). -/
+private
+def ppArray [ToString α]
+  (array : Array α)
+  (sep : String := ", ")
+  (delim : String × String := ("#[", "]"))
+: String := Id.run do
+  let mut s := ""
+  for elm in array do
+    if ¬ s.isEmpty then
+      s := s ++ sep
+    s := s ++ toString elm
+  delim.1 ++ s ++ delim.2
+
+/-- info:
+#[1, 2, 3]
+#[1 - 2 - 3]
+<| 1 | 2 | 3 |>
+<| 1 | 2 | 3 |>
+⟦1 · 2 · 3⟧
+-/
+#guard_msgs in #eval do
+  let array := #[1, 2, 3]
+  println! "{ppArray array}"
+  let s := ppArray array " - "
+  println! "{s}"
+  let s := ppArray array " | " ("<| ", " |>")
+  println! "{s}"
+  let s := ppArray array " | " ("<| ", " |>")
+  println! "{s}"
+  let s := ppArray (delim := ("⟦", "⟧")) (sep := " · ") array
+  println! "{s}"
+
+
+
+/-! ## Monad transformers
+
+Now, what if we want a state monad that allows operations from other monads such as `IO`, or the
+*result* monad `Except ε`?
+-/
+
+abbrev BadSMonT (σ : Type) (M : Type → Type) (α : Type) : Type :=
+  M (σ → α × σ)
+
+abbrev SMonT (σ : Type) (M : Type → Type) (α : Type) : Type :=
+  σ → M (α × σ)
+
+namespace SMonT
+instance instMonad [Monad M] : Monad (SMonT σ M) where
+  pure a state := pure (a, state)
+  bind a? f? state := do
+    let (a, state) ← a? state
+    f? a state
+
+variable [Monad M]
+
+/-! Write the following functions. -/
+section sol!
+def get : SMonT σ M σ
+| state => return (state, state)
+
+def set (state : σ) : SMonT σ M Unit
+| _oldState => return ((), state)
+
+def printState [ToString σ] : SMonT σ IO Unit
+| state => do
+  println! "state: {state}"
+  return ((), state)
+end sol!
+
+/-- info: Zen.Train.Trash.SMonT.get {M : Type → Type} [Monad M] {σ : Type} : SMonT σ M σ -/
+#guard_msgs in #check get
+/-- info:
+Zen.Train.Trash.SMonT.set {M : Type → Type} [Monad M] {σ : Type} (state : σ) : SMonT σ M Unit
+-/
+#guard_msgs in #check set
+/-- info: Zen.Train.Trash.SMonT.printState {σ : Type} [ToString σ] : SMonT σ IO Unit -/
+#guard_msgs in #check printState
+
+/-- info:
+state: 7
+final state is `7`
+-/
+#guard_msgs in #eval do
+  let state := 7
+  let (_, state) ← printState state
+  println! "final state is `{state}`"
+
+
+
+/-! It's tedious to have to "deconstruct" our monad transformer to run `M`-code.
+
+Check out this class, and write the appropriate instance.
+-/
+#checkout MonadLift
+
+section sol!
+instance instMonadLift : MonadLift M (SMonT σ M) where
+  monadLift a? state := do
+    let a ← a?
+    return (a, state)
+end sol!
+
+/-! This gives access to `liftM` which (here) can lift `IO`-code to `SMonT σ IO`-code. -/
+
+def printState' [ToString σ] : SMonT σ IO Unit := do
+  let state ← get
+  liftM $ println! "state: {state}"
+
+/-- info:
+state: 7
+final state is `7`
+-/
+#guard_msgs in #eval do
+  let state := 7
+  let (_, state) ← printState' state
+  println! "final state is `{state}`"
+
+
+
+/-! What if `M` is not really `IO`, but just something that `MonadLift`-s from `IO`? -/
+def printState'' [MonadLift IO M] [ToString σ] : SMonT σ M Unit := do
+  let state ← get
+  liftM $ println! "state: {state}"
+
+/-! This is too easy, now we can write functions like these. Right? -/
+
+/-- error:
+failed to synthesize instance
+  MonadLift IO IO
+-/
+#guard_msgs in
+def printState''IO [ToString σ] : SMonT σ IO Unit :=
+  printState''
+
+/-! We can't 🙀
+
+Let's actually check `liftM`'s type:
+-/
+#checkout liftM
+/-! which leads us to: -/
+#checkout MonadLiftT
+
+/-! Let's try this again. -/
+def printState''' [MonadLiftT IO M] [ToString σ] : SMonT σ M Unit := do
+  let state ← get
+  liftM $ println! "state: {state}"
+
+def printState'''IO [ToString σ] : SMonT σ IO Unit :=
+  printState'''
+
+/-! Nice. -/
+
+end SMonT
