Bf/Part4.lean
@@ -2,8 +2,17 @@ import Bf.Part3
 
 
 
+/-! # Metaprogramming
+
+Metaprogramming in Lean 4 is **deep**: Lean 4 is a reflexive language 🙀
+
+- <https://leanprover-community.github.io/lean4-metaprogramming-book/main/01_intro.html>
+-/
 namespace Zen.Train.Bf
 
+
+
+namespace Dsl
 
 
 
@@ -28,15 +37,15 @@ syntax "." : brnfck
 syntax ".." : brnfck
 syntax "," : brnfck
 
-syntax "[" brnfck "]" : brnfck
-syntax "[" "]" : brnfck
+syntax "[" brnfck ? "]" : brnfck
 syntax brnfck brnfck : brnfck
 syntax "![" term "]" : brnfck
-syntax "echo!" "(" term ")" : brnfck
-syntax "check!" "(" term "," term ")" : brnfck
+syntax "dbg!" "(" term ")" : brnfck
+syntax "chk!" "(" term "," term ")" : brnfck
 
 
 
+/-- Syntax extension to create `Bf.Ast`-s. -/
 syntax "Bf.ast!" "(" brnfck ")" : term
 
 macro_rules
@@ -66,88 +75,197 @@ macro_rules
   ``( Ast.chain Bf.ast!($fst) Bf.ast!($snd) )
 | `( Bf.ast!( ![$t] ) ) =>
   ``($t)
-| `( Bf.ast!( echo!($s) ) ) =>
+| `( Bf.ast!( dbg!($s) ) ) =>
   ``(Ast.dbg $s)
-| `( Bf.ast!( check!($val, $msg) ) ) =>
+| `( Bf.ast!( chk!($val, $msg) ) ) =>
   ``(Ast.chk $val $msg)
+
+example : Bf.ast!(.) = Ast.out :=
+  rfl
+example : Bf.ast!(..) = Ast.seqN 2 .out :=
+  rfl
+example : Bf.ast!(—.) = Ast.seq #[.dec, .out] :=
+  rfl
+
+/-- info: >.,[],,..++----- -/
+#guard_msgs in #eval Bf.ast!(>.,[],,..++—————)
+/-- info: >.,[],,.[.++>----].++----- -/
+#guard_msgs in #eval
+  let someCode := Bf.ast!([.++>————])
+  Bf.ast!(>.,[],,.![someCode].++—————)
+
+/-- info: #[8] -/
+#guard_msgs in #eval
+  Bf.ast!(,[->+<]>.).evalTo! [8] .array
+
+/-- info:
+entering loop
+exiting loop
+#[4]
+-/
+#guard_msgs in #eval
+  Bf.ast!(
+    ++++
+    dbg!("entering loop")
+    [->+<]
+    dbg!("exiting loop")
+    >.
+    chk!(4, "not 4 :/")
+  ).evalIO! []
+
+/-- info:
+#[4]
+-/
+#guard_msgs in #eval
+  Bf.ast!(
+    ++++
+    dbg!("entering loop")
+    [->+<]
+    dbg!("exiting loop")
+    >.
+    chk!(4, "not 4 :/")
+  ).eval! []
+
+end Dsl
+
+
+
+namespace Rt
+
+def BfT.handleSeffElab : Ast.Seff → BfT Lean.Elab.Term.TermElabM Unit
+| .dbg msg => do
+  Lean.logInfo msg
+| seff =>
+  handleSeff seff
+
+protected instance Elab : Spec (BfT Lean.Elab.Term.TermElabM) :=
+  { Rt.NoIO with seff := BfT.handleSeffElab }
+
+def Spec.runExtractExpr
+  [Monad M] [Inhabited α] [Lean.ToExpr α]
+  (S : Spec (BfT M)) (code : Ast) (inputs : List Nat) (ex : Extract α)
+: M (BfT.Res Lean.Expr) := do
+  let res ← S.exe code inputs ex
+  return Lean.ToExpr.toExpr <$> res
+
+end Rt
+
+
+
+namespace Dsl
+
+
+
+declare_syntax_cat brnfckRunOpt
+
+syntax "-q" : brnfckRunOpt
+syntax "-quiet" : brnfckRunOpt
+syntax "-no-check" : brnfckRunOpt
+syntax "-no-loop-limit" : brnfckRunOpt
+syntax "-loop-limit" term:max : brnfckRunOpt
+
+inductive RunOpt
+| quiet
+| noCheck
+| loopLimit : Option Nat → RunOpt
+
+namespace RunOpt
+
+open Lean (TSyntax)
+open Lean.Elab
+
+unsafe def ofStx : TSyntax `brnfckRunOpt → TermElabM RunOpt
+| `(brnfckRunOpt| -q)
+| `(brnfckRunOpt| -quiet) => return quiet
+| `(brnfckRunOpt| -no-check) => return noCheck
+| `(brnfckRunOpt| -no-loop-limit) => return loopLimit none
+| `(brnfckRunOpt| -loop-limit $l) => do
+  let l ← Term.evalTerm Nat (Lean.mkConst ``Nat) l
+  return loopLimit l
+| _ => throwUnsupportedSyntax
+
+def apply (config : Rt.Config) : RunOpt → Rt.Config
+| quiet => {config with dbg := false}
+| noCheck => {config with check := false}
+| loopLimit l => {config with loopLimit := l}
+
+unsafe def handleStxArray (opts : Array (TSyntax `brnfckRunOpt)) : TermElabM Rt.Config := do
+  let mut conf := Rt.Config.default
+  for opt in ← opts.mapM ofStx do
+    conf := opt.apply conf
+  return conf
+end RunOpt
+
+
+
+/-- `Bf.run! [extractor] ast [inputs]`
+
+Runs `ast` with optionals `inputs`, and runs the optional `extractor` (`Extractor.array` if none).
+-/
+syntax (name := Bf.run)
+  "Bf.run!" (brnfckRunOpt)*
+    ("[" term "]")?
+    "(" brnfck ")"
+    ("[" term "]")?
+: term
 
 
 
 section elab!
-  syntax (name := Bf.run)
-    "Bf.run!"
-        ("[" term "]")?
-        "(" brnfck ")"
-        ("[" term "]")?
-  : term
 
-  open Lean.Elab.Term (TermElab evalTerm)
-  open Lean (mkApp mkConst levelZero)
+open Lean.Elab.Term (TermElab evalTerm)
+open Lean (mkApp mkConst levelZero)
 
-  def typExtract' := mkConst ``Rt.Extract'
-  def typNat := mkConst ``Nat
-  def typAst := mkConst ``Ast
-  def typArrayNat := mkApp (mkConst ``Array [levelZero]) typNat
-  def typIOArrayNat := mkApp (mkConst ``IO []) typArrayNat
-  def typExpr := mkConst ``Lean.Expr []
-  def typIOExpr := mkApp (mkConst ``IO []) typExpr
-  def typIOResExpr := mkApp (mkConst ``IO []) (mkApp (mkConst ``Rt.BfT.Res []) typExpr)
-  def typListNat := mkApp (mkConst ``List [levelZero]) typNat
+def typNat := mkConst ``Nat
+def typExpr := mkConst ``Lean.Expr
+def typElabResExpr := mkApp (mkConst ``Lean.Elab.TermElabM) (mkApp (mkConst ``Rt.BfT.Res) typExpr)
+def typListNat := mkApp (mkConst ``List [levelZero]) typNat
 
-  @[term_elab Bf.run]
-  unsafe def elabBfRun : TermElab := fun stx _expectedType? =>
-    match stx with
-    | `(
-      Bf.run!
-        $[[$ex:term]]?
-        ($ast:brnfck)
-        $[[$inputs:term]]?
-    ) => do
-      let inputs :=
-        if let some inputs := inputs
-        then inputs else ← `([])
-      let ex ←
-        if let some ex := ex then pure ex else `(Rt.Extract.array)
-      let toRun ← `(Rt.BfT.justRunToExpr Rt.BfT.instSpecIO (M := IO) Bf.ast!($ast) $inputs $ex)
-      let expr ← Lean.Elab.Term.elabTerm toRun none
-      Lean.Elab.Term.synthesizeSyntheticMVarsNoPostponing
-      let expr ← Lean.instantiateMVars expr
-      let ioExpr? ← Lean.Meta.evalExpr (IO (Rt.BfT.Res Lean.Expr)) typIOResExpr expr
-      let expr? ← ioExpr?
-      match expr? with
-      | .ok res _ => return res
-      | .error e state =>
-        let mem := state.mem.mapIdx fun idx val =>
-          if idx = state.ptr then s!"*{val}*" else toString val
-        IO.throwServerError s!"\
-{e.toString}
-- memory: {mem}\
-        "
-    | _ => Lean.Elab.throwUnsupportedSyntax
+@[term_elab Bf.run]
+unsafe def elabBfRun : TermElab := fun stx _expectedType? =>
+  match stx with
+  | `(
+    Bf.run!
+      -- $[$opts:brnfckRunOpt]*
+      $[[$ex:term]]? ($ast:brnfck) $[[$inputs:term]]?
+  ) => do
+    -- let conf ← RunOpt.handleStxArray opts
+    let inputs :=
+      if let some inputs := inputs
+      then inputs else ← `([])
+    let ex ←
+      if let some ex := ex then pure ex else ``(Rt.Extract.array)
+    let toRun ← ``(Rt.Elab.runExtractExpr Bf.ast!($ast) $inputs $ex)
+    let expr ← Lean.Elab.Term.elabTerm toRun none
+    Lean.Elab.Term.synthesizeSyntheticMVarsNoPostponing
+    let expr ← Lean.instantiateMVars expr
+    let elabExpr ←
+      Lean.Meta.evalExpr (Lean.Elab.TermElabM (Rt.BfT.Res Lean.Expr)) typElabResExpr expr
+    let expr? ← elabExpr
+    match expr? with
+    | .ok res _ => return res
+    | .error e state =>
+      let mem := state.mem.mapIdx fun idx val =>
+        if idx = state.ptr then s!"*{val}*" else toString val
+      Lean.throwError m!"{e.toString}\n- memory: {mem}"
+  | _ => Lean.Elab.throwUnsupportedSyntax
 end elab!
 
-#eval println! "=> `{Bf.ast!(..)}`"
-example : Bf.ast!(.) = Ast.out :=
-  rfl
-
-#eval println! "=> `{Bf.ast!(+ +)}`"
-example : Bf.ast!(—.) = Ast.seq #[.dec, .out] :=
-  rfl
-
-#eval
-  let blah := Ast.Test.val1
-  Bf.ast!(++![blah])
-
-#check Bf.run!(+++.)
 example : Bf.run!(+++.) = #[3] := by
   rfl
 
+/-- info:
+done
+-/
+#guard_msgs in example : Bf.run!(![Ast.Test.val1]) = #[2] := by
+  rfl
+
 /-- error:
-value check failed, expected `7`, got `3`: not 7 :/
-- memory: #[*3*]
+value check failed, expected `7`, got `3`: not `7` :/
+- memory: [*3*]
 -/
 #guard_msgs in #eval
-  Bf.run![.array](+++.check!(7, "not 7 :/"))
+  Bf.run![.array](+++.chk!(7, "not `7` :/"))
 
 example : Bf.run![.head?](+++.) = some 3 :=
   rfl
@@ -171,46 +289,24 @@ I 🖤 catz
     println! s
 
 /-- error:
-error: [bf] failed to extract output `head!`, no output available
-- memory: #[*3*]
+[bf] failed to extract output `head!`, no output available
+- memory: [*3*]
 -/
 #guard_msgs in #eval
   Bf.run![.head!](+++)
 
 
 example : Bf.run![.head!](
-  check!(0, "@0 is 0 on init")
+  chk!(0, "@0 is 0 on init")
   +++++++
-  check!(7, "added 1 × 7 to @0")
+  chk!(7, "added 1 × 7 to @0")
   [->+<]>
-  check!(7, "copied 7@0 to @1")
+  chk!(7, "copied 7@0 to @1")
   .
 ) = 7 :=
   rfl
-
-#check Bf.ast!(.)
-#eval Bf.ast!(>.,[],,..++—————)
-#eval Rt.NoIO.justRun! (M := Id) Bf.ast!(,[->+<]>.) [8] .array
-#eval
-  let someCode := Bf.ast!([.++>————])
-  Bf.ast!(>.,[],,.![someCode].++—————)
 
 #eval
   Bf.run!(+++.)
 #eval
   Bf.run!(, +++.)
-
-/-- info:
-entering loop
-exiting loop
-#[4]
--/
-#guard_msgs in #eval
-  Bf.ast!(
-    ++++
-    echo!("entering loop")
-    [->+<]
-    echo!("exiting loop")
-    >.
-    check!(4, "not 4 :/")
-  ).evalIO! []
